ulib/prims.fst
@@ -20,11 +20,11 @@ assume type hasEq: Type -> GTot Type0
 
 type eqtype = a:Type{hasEq a}
 
-(* False is the empty inductive type *)
-type c_False =
+(* Constructive False is the empty inductive type *)
+type c_false : Type0 =
 
-(* True is the singleton inductive type *)
-type c_True =
+(* Constructive True is the singleton inductive type *)
+type c_true : Type0 =
   | T
 
 (* another singleton type, with its only inhabitant written '()'
@@ -32,40 +32,32 @@ type c_True =
 assume new type unit : Type0
 assume HasEq_unit: hasEq unit
 
-(* A coercion down to universe 0 *)
+(* Squash is a coercion down to universe 0
+   (i.e. a proof irrelevant type) *)
 type squash (p:Type) : Type0 = x:unit{p}
 
-(*
- * Squashed versions of truth and falsehood
- *)
-type l_True = squash c_True
-type l_False = squash c_False
+(* Squashed versions of truth and falsehood *)
+type l_true : Type0 = squash c_true
+type l_false : Type0 = squash c_false
 
 (* An SMT-pattern to control unfolding inductives;
    In a proof, you can say `allow_inversion (option a)`
-   to allow the SMT solver. cf. allow_inversion below
- *)
-let inversion (a:Type) = True
+   to allow the SMT solver. cf. allow_inversion below  *)
+let inversion (a:Type) : Type0 = l_true
 
-(* The usual equality deifned as an inductive type *)
-type equals (#a:Type) (x:a) : a -> Type =
-  | Refl : equals x x
-  
-(* infix binary '==';
-   proof irrelevant, heterogeneous equality in Type#0
-*)   
-//TODO: instead of hard-wiring the == syntax, 
-//       we should just rename eq2 to op_Equals_Equals
-type eq2 (#a:Type) (x:a) (y:a) = squash (equals x y)
+(* Constructive Leibniz equality (i.e. homogeneous) defined as inductive type *)
+type c_equals (#a:Type) (x:a) : a -> Type =
+  | Refl : c_equals x x
 
-(* Heterogeneous equality *)
-type h_equals (#a:Type) (x:a) : #b:Type -> b -> Type = 
-  | HRefl : h_equals x x
+(* Squashed Leibniz equality (i.e. homogeneous) *)
+type l_equals (#a:Type) (x:a) (y:a) = squash (c_equals x y)
 
-(* A proof-irrelevant version of h_equals *)
-type eq3 (#a:Type) (#b:Type) (x:a) (y:b) = squash (h_equals x y)
+(* Constructive heterogeneous equality *)
+type c_hequals (#a:Type) (x:a) : #b:Type -> b -> Type =
+  | HRefl : c_hequals x x
 
-unfold let op_Equals_Equals_Equals (#a:Type) (#b:Type) (x:a) (y:b) = eq3 x y
+(* Squashed heterogeneous equality *)
+type l_hequals (#a:Type) (#b:Type) (x:a) (y:b) : Type0 = squash (c_hequals x y)
 
 (* bool is a two element type with elements {'true', 'false'}
    we assume it is primitive, for convenient interop with other languages *)
@@ -76,43 +68,60 @@ assume HasEq_bool: hasEq bool
 type b2t (b:bool) = (b == true)
 
 (* constructive conjunction *)
-type c_and  (p:Type) (q:Type) =
+type c_and  (p:Type) (q:Type) : Type =
   | And   : p -> q -> c_and p q
 
-(* '/\'  : specialized to Type#0 *)
-type l_and (p:Type0) (q:Type0) = squash (c_and p q)
+(* squashed conjunction *)
+type l_and (p:Type0) (q:Type0) : Type0 = squash (c_and p q)
 
 (* constructive disjunction *)
-type c_or   (p:Type) (q:Type) =
+type c_or   (p:Type) (q:Type) : Type =
   | Left  : p -> c_or p q
   | Right : q -> c_or p q
 
-(* '\/'  : specialized to Type#0 *)
-type l_or (p:Type0) (q:Type0) = squash (c_or p q)
+(* squashed disjunction *)
+type l_or (p:Type0) (q:Type0) : Type0 = squash (c_or p q)
 
-(* '==>' : specialized to Type#0 *)
-type l_imp (p:Type0) (q:Type0) = squash (p -> GTot q)
-                                         (* ^^^ NB: The GTot effect is primitive;            *)
-				         (*         elaborated using GHOST a few lines below *)
-(* infix binary '<==>' *)
-type l_iff (p:Type) (q:Type) = (p ==> q) /\ (q ==> p)
+(* constructive implication *)
+type c_imp (p:Type) (q:Type) : Type = (p -> GTot q)
 
-(* prefix unary '~' *)
-type l_not (p:Type) = l_imp p False
+(* squashed implication *)
+type l_imp (p:Type0) (q:Type0) : Type0
+  = squash (p -> GTot q)
+               (* ^^^ NB: The GTot effect is primitive;            *)
+               (*         elaborated using GHOST a few lines below *)
 
-unfold type l_ITE (p:Type) (q:Type) (r:Type) = (p ==> q) /\ (~p ==> r)
+(* constructive equivalence *)
+type c_iff (p:Type) (q:Type) : Type = c_and (c_imp p q) (c_imp q p)
+
+(* squashed equivalence *)
+type l_iff (p:Type0) (q:Type0) : Type0 = l_and (l_imp p q) (l_imp q p)
+
+(* constructive not *)
+type c_not (p:Type) : Type = c_imp p c_false
+
+(* squashed not *)
+type l_not (p:Type0) : Type0 = l_imp p l_false
+
+(* squashed if-then-else *)
+unfold type l_ite (p:Type0) (q:Type0) (r:Type0) : Type0
+  = l_and (l_imp p q) (l_imp (l_not p) r)
 
 (* infix binary '<<'; a built-in well-founded partial order over all terms *)
 assume type precedes : #a:Type -> #b:Type -> a -> b -> Type0
 
 (* internalizing the typing relation for the SMT encoding: (has_type x t) *)
 assume type has_type : #a:Type -> a -> Type -> Type0
-  
-(* forall (x:a). p x : specialized to Type#0 *)
-type l_Forall (#a:Type) (p:a -> GTot Type0) = squash (x:a -> GTot (p x))
 
-(* The type of squashed types *)
-type prop = a:Type0{ forall (x:a) (y:a). x == y }
+(* constructive forall *)
+type c_forall (#a:Type) (p:a -> GTot Type) : Type = (x:a -> GTot (p x))
+
+(* squashed forall *)
+type l_forall (#a:Type) (p:a -> GTot Type0) : Type0 = squash (x:a -> GTot (p x))
+
+(* The type of propositions (types with at most one inhabitant)
+   It's trivial to show that all squashed types are in prop *)
+type prop = a:Type0{ l_forall #a (fun x -> l_forall #a (fun y -> l_equals x y)) }
 
 (* dependent pairs DTuple2 in concrete syntax is '(x:a & b x)' *)
 unopteq type dtuple2 (a:Type)
@@ -121,8 +130,11 @@ unopteq type dtuple2 (a:Type)
             -> _2:b _1
             -> dtuple2 a b
 
-(* exists (x:a). p x : specialized to Type#0 *)
-type l_Exists (#a:Type) (p:a -> GTot Type0) = squash (x:a & p x)
+(* constructive exists *)
+type c_exists (#a:Type) (p:a -> GTot Type) : Type = (x:a & p x)
+
+(* squashed exists *)
+type l_exists (#a:Type) (p:a -> GTot Type0) : Type0 = squash (x:a & p x)
 
 assume new type range : Type0
 assume val range_0:range
@@ -148,7 +160,7 @@ unfold let pure_bind_wp (r1:range) (a:Type) (b:Type)
                    (p : pure_post b) =
 	wp1 (fun (x:a) -> wp2 x p)
 unfold let pure_if_then_else (a:Type) (p:Type) (wp_then:pure_wp a) (wp_else:pure_wp a) (post:pure_post a) =
-     l_ITE p (wp_then post) (wp_else post)
+     l_ite p (wp_then post) (wp_else post)
 
 unfold let pure_ite_wp (a:Type) (wp:pure_wp a) (post:pure_post a) =
      forall (k:pure_post a).
@@ -227,8 +239,8 @@ type list (a:Type) =
 
 noeq type pattern =
   | SMTPat   : #a:Type -> a -> pattern
-  | SMTPatT  : a:Type0 -> pattern 
-  | SMTPatOr : list (list pattern) -> pattern 
+  | SMTPatT  : a:Type0 -> pattern
+  | SMTPatOr : list (list pattern) -> pattern
 
 assume type decreases : #a:Type -> a -> Type0
 
@@ -277,8 +289,8 @@ let st_wp_h   (heap:Type) (a:Type) = st_post_h heap a -> Tot (st_pre_h heap)
 unfold let st_return        (heap:Type) (a:Type)
                             (x:a) (p:st_post_h heap a) =
      p x
-unfold let st_bind_wp       (heap:Type) 
-			    (r1:range) 
+unfold let st_bind_wp       (heap:Type)
+			    (r1:range)
 			    (a:Type) (b:Type)
                             (wp1:st_wp_h heap a)
                             (wp2:(a -> GTot (st_wp_h heap b)))
@@ -287,7 +299,7 @@ unfold let st_bind_wp       (heap:Type)
 unfold let st_if_then_else  (heap:Type) (a:Type) (p:Type)
                              (wp_then:st_wp_h heap a) (wp_else:st_wp_h heap a)
                              (post:st_post_h heap a) (h0:heap) =
-     l_ITE p
+     l_ite p
         (wp_then post h0)
 	(wp_else post h0)
 unfold let st_ite_wp        (heap:Type) (a:Type)
@@ -353,7 +365,7 @@ unfold let ex_ite_wp (a:Type) (wp:ex_wp a) (post:ex_post a) =
      ==> wp k
 
 unfold let ex_if_then_else (a:Type) (p:Type) (wp_then:ex_wp a) (wp_else:ex_wp a) (post:ex_post a) =
-   l_ITE p
+   l_ite p
        (wp_then post)
        (wp_else post)
 unfold let ex_stronger (a:Type) (wp1:ex_wp a) (wp2:ex_wp a) =
@@ -407,7 +419,7 @@ unfold let all_bind_wp (heap:Type) (r1:range) (a:Type) (b:Type)
 unfold let all_if_then_else (heap:Type) (a:Type) (p:Type)
                              (wp_then:all_wp_h heap a) (wp_else:all_wp_h heap a)
                              (post:all_post_h heap a) (h0:heap) =
-   l_ITE p
+   l_ite p
        (wp_then post h0)
        (wp_else post h0)
 unfold let all_stronger (heap:Type) (a:Type) (wp1:all_wp_h heap a)
@@ -613,3 +625,51 @@ abstract let normalize (a:Type0) = a
 
 val assert_norm : p:Type -> Pure unit (requires (normalize p)) (ensures (fun _ -> p))
 let assert_norm p = ()
+
+(*********************************************************************************)
+(* Propositional logical connectives *)
+(*********************************************************************************)
+
+(* prop truth and falsehood *)
+let p_true : (* Tot *) prop = l_true
+let p_false : (* Tot *) prop = l_false
+
+(* prop homogeneous equality *)
+let p_equals (#a:Type) (x:a) (y:a) : Tot prop = l_equals x y
+
+(* infix binary '==' *)
+unfold let op_Equals_Equals (#a:Type) (x:a) (y:a) : Tot prop
+  = p_equals x y
+
+(* prop heterogeneous equality *)
+let p_hequals (#a:Type) (#b:Type) (x:a) (y:b) : Tot prop
+  = l_hequals x y
+
+(* infix binary '===' *)
+unfold let op_Equals_Equals_Equals (#a:Type) (#b:Type) (x:a) (y:b) : Tot prop
+  = p_hequals x y
+
+(* bool-to-prop coercion *)
+(* type b2p (b:bool) : prop = b2t b -- doesn't work, `logical` crap? *)
+let b2p (b:bool) : prop = (b == true)
+
+(* infix binary '/\': prop conjunction *)
+let p_and (p:prop) (q:prop) : Tot prop = l_and p q
+
+(* infix binary '\/': prop implication *)
+let p_or (p:prop) (q:prop) : Tot prop = l_or p q
+
+(* infix binary '==>': prop implication *)
+let p_imp (p:prop) (q:prop) : Tot prop = l_imp p q
+
+(* infix binary '<==>': prop equivalence *)
+let p_iff (p:prop) (q:prop) : Tot prop = l_iff p q
+
+(* prefix unary '~' *)
+let p_not (p:prop) : Tot prop = l_not p
+
+(* forall (x:a). p x : prop forall *)
+let p_forall (#a:Type) (p:a -> GTot prop) : Tot prop = l_forall #a p
+
+(* exists (x:a). p x : prop exists *)
+let p_exists (#a:Type) (p:a -> GTot prop) : Tot prop = l_exists #a p
